Test/dafny0/runtest.bat
@@ -12,7 +12,7 @@ for %%f in (Simple.dfy) do (
 )
 
 for %%f in (TypeTests.dfy NatTypes.dfy SmallTests.dfy Definedness.dfy
-            FunctionSpecifications.dfy ResolutionErrors.dfy
+            FunctionSpecifications.dfy ResolutionErrors.dfy ParseErrors.dfy
             Array.dfy MultiDimArray.dfy NonGhostQuantifiers.dfy AdvancedLHS.dfy
             Modules0.dfy Modules1.dfy BadFunction.dfy
             Comprehensions.dfy Basics.dfy ControlStructures.dfy
